chacha20 using layered effects (taken from Aymeric's branch)

examples/layeredeffects/RST.Effect.Test.fst
@@ -35,56 +35,33 @@ open RST.Effect
   -LowStar \
   -FStar.ModifiesGen'"
 
-assume val r1 : r:resource{r.t == nat}
-
-assume val test5 (x:int)
-: RST unit r1 (fun _ -> r1)
-  (fun _ -> x > 0)
-  (fun _ _ _ -> True)
-
-#set-options "--debug RST.Effect.Test --debug_level Rel --debug_level Extreme --print_full_names --print_universes --ugly --debug_level TwoPhases --debug_level LayeredEffects --print_implicits --print_bound_var_types --debug_level SMTEncoding --debug_level SMTQuery" //--print_effect_args"
-
-//[@expect_failure]
-
-#restart-solver
-#set-options "--log_queries"
-
-let test6 (l:list int)
-: RST unit r1 (fun _ -> r1)
-  (fun _ -> Cons? l /\ Cons?.hd l > 0)
-  (fun _ _ _ -> True)
-= match l with
-  | hd::_ -> test5 hd
-
-
 // (*
-//  * This code doesn't typecheck without the <: Tot nat ascription
-//  * What happens is:
-//  *   We first typecheck 2 : Tot int
-//  *   Then the expected type in the environment is nat (coming from the return type annotation)
-//  *   So we check that (2 : int <: nat)
-//  *   This succeeds with guard (2 >= 0),
-//  *   But in the process we end up inserting a return and make (2 : PURE nat (pure_return_wp int 2))
-//  *   Note the type int in the pure_return_wp -- this is because we end up using the initial type
-//  *   (TcTerm.value_check_expected_type - call to TcUtil.return_value)
-//  *
-//  *   Now the problem is, when we lift PURE nat (pure_return_wp int 2) to RST,
-//  *     the unification happens at type nat,
-//  *     and we unify (pure_return_wp int 2) to the (wp:pure_wp nat) argument of lift
-//  *     and this fails to typecheck (generates an smt query that forall (x:int). x >= 0)
-//  *
-//  *   Adding the (Tot nat) ascription ensures that the return is inserted at type nat, and then we are good
-//  *
-//  *   We need to figure out a way to handle this, not typecheck these binders in layered effect combinators?
-//  *)
+// //  * This code doesn't typecheck without the <: Tot nat ascription
+// //  * What happens is:
+// //  *   We first typecheck 2 : Tot int
+// //  *   Then the expected type in the environment is nat (coming from the return type annotation)
+// //  *   So we check that (2 : int <: nat)
+// //  *   This succeeds with guard (2 >= 0),
+// //  *   But in the process we end up inserting a return and make (2 : PURE nat (pure_return_wp int 2))
+// //  *   Note the type int in the pure_return_wp -- this is because we end up using the initial type
+// //  *   (TcTerm.value_check_expected_type - call to TcUtil.return_value)
+// //  *
+// //  *   Now the problem is, when we lift PURE nat (pure_return_wp int 2) to RST,
+// //  *     the unification happens at type nat,
+// //  *     and we unify (pure_return_wp int 2) to the (wp:pure_wp nat) argument of lift
+// //  *     and this fails to typecheck (generates an smt query that forall (x:int). x >= 0)
+// //  *
+// //  *   Adding the (Tot nat) ascription ensures that the return is inserted at type nat, and then we are good
+// //  *
+// //  *   We need to figure out a way to handle this, not typecheck these binders in layered effect combinators?
+// //  *)
 // let test1 ()
 // : RST nat emp (fun _ -> emp) (fun _ -> True) (fun _ r _ -> r == 2)
-// = (2 <: Tot nat)
+// = 2
 
-
+// assume val r1 : r:resource{r.t == nat}
 // assume val r2 : r:resource{r.t == nat}
 // assume val r3 : r:resource{r.t == nat}
-
 
 // assume val f1
 // : x:nat ->
@@ -149,3 +126,219 @@ let test6 (l:list int)
 
 // /// Testing basic pattern matching
 
+// assume val test5 (x:int)
+// : RST unit r1 (fun _ -> r1)
+//   (fun _ -> x > 0)
+//   (fun _ _ _ -> True)
+
+// let test6 (l:list int)
+// : RST unit r1 (fun _ -> r1)
+//   (fun _ -> Cons? l /\ Cons?.hd l > 0)
+//   (fun _ _ _ -> True)
+// = match l with
+//   | hd::_ -> test5 hd
+
+ 
+(*** chacha20 ***)
+
+/// The effect definitions and `rst_frame` are as defined in `examples/layered_effect/RST.Effect.fst`
+
+module U32 = FStar.UInt32
+
+assume val array (a:Type0) : Type0
+assume val length (#a:Type0) (b:array a) : nat
+assume val array_resource (#a:Type0) (b:array a) : resource
+assume val as_rseq (#a:Type0) (b:array a) (#r:resource{array_resource b `is_subresource_of` r}) (h:rmem r)
+: GTot (s:Seq.seq a{Seq.length s == length b})
+
+assume val index (#a:Type0) (b:array a) (i:U32.t{U32.v i < length b})
+: unit ->
+  RST a
+  (array_resource b)
+  (fun _ -> array_resource b)
+  (fun _ -> True)
+  (fun h0 x h1 ->
+    x == Seq.index (as_rseq b h0) (U32.v i) /\
+    h0 == h1)
+
+assume val upd (#a:Type0) (b:array a) (i:U32.t{U32.v i < length b}) (v:a)
+: unit ->
+  RST unit
+  (array_resource b)
+  (fun _ -> array_resource b)
+  (fun _ -> True)
+  (fun h0 _ h1 ->
+    let s0 = as_rseq b h0 in
+    let s1 = as_rseq b h1 in
+    Seq.index s1 (U32.v i) == v /\
+    (forall (j:nat).{:pattern Seq.index s1 j} (j < Seq.length s1 /\ j =!= (U32.v i)) ==>
+              (Seq.index s1 j == Seq.index s0 j)))
+
+
+type state = b:array U32.t{length b == 16}
+
+assume val rst_get (r:resource)
+: RST (rmem r)
+  r (fun _ -> r)
+  (fun _ -> True)
+  (fun h0 r h1 -> r == h0 /\ h1 == h0)
+
+
+/// `focus_rmem` doesn't work well for me, so adding lemmas that I need for chacha20 function below
+
+assume val as_rseq_focus_rmem1 (#a:Type0)
+  (b1 b2:array a) (h:rmem (array_resource b1 <*> array_resource b2))
+: Lemma (as_rseq b1 h == as_rseq b1 (focus_rmem h (array_resource b1)))
+        [SMTPat (as_rseq b1 h)]
+
+assume val as_rseq_focus_rmem2 (#a:Type0)
+  (b1 b2:array a) (h:rmem (array_resource b1 <*> array_resource b2))
+: Lemma (as_rseq b2 h == as_rseq b2 (focus_rmem h (array_resource b2)))
+        [SMTPat (as_rseq b2 h)]
+
+assume val as_rseq_focus_rmem_inv1 (#a:Type0)
+  (b1 b2:array a) (h0 h1:rmem (array_resource b1 <*> array_resource b2))
+: Lemma
+  (requires focus_rmem h0 (array_resource b1) == focus_rmem h1 (array_resource b1))
+  (ensures as_rseq b1 h0 == as_rseq b1 h1)
+  [SMTPat (focus_rmem h0 (array_resource b1)); SMTPat (focus_rmem h1 (array_resource b1))]
+
+assume val as_rseq_focus_rmem_inv2 (#a:Type0)
+  (b1 b2:array a) (h0 h1:rmem (array_resource b1 <*> array_resource b2))
+: Lemma
+  (requires focus_rmem h0 (array_resource b2) == focus_rmem h1 (array_resource b2))
+  (ensures as_rseq b2 h0 == as_rseq b2 h1)
+  [SMTPat (focus_rmem h0 (array_resource b2)); SMTPat (focus_rmem h1 (array_resource b2))]
+
+
+/// `copy_state`
+
+#set-options "--max_fuel 0 --max_ifuel 0"
+let copy_state
+  (st:state)
+  (ost:state)
+: RST unit
+  (array_resource st <*> array_resource ost)
+  (fun _ -> array_resource st <*> array_resource ost)
+  (fun _ -> True)
+  (fun h0 _ h1 ->
+    focus_rmem h0 (array_resource ost) == focus_rmem h1 (array_resource ost) /\
+    as_rseq st h1 `Seq.equal` as_rseq ost h0)
+= let both_st = array_resource st <*> array_resource ost in
+  let h0 = rst_get both_st in
+  let v =
+    rst_frame both_st (fun _ -> both_st) (array_resource st)
+    (index ost 0ul) in
+
+  rst_frame both_st (fun _ -> both_st) (array_resource ost)
+    (upd st 0ul v);
+
+  let v =
+    rst_frame both_st (fun _ -> both_st) (array_resource st)
+    (index ost 1ul) in
+
+  rst_frame both_st (fun _ -> both_st) (array_resource ost)
+    (upd st 1ul v);
+
+  let v =
+    rst_frame both_st (fun _ -> both_st) (array_resource st)
+    (index ost 2ul) in
+
+  rst_frame both_st (fun _ -> both_st) (array_resource ost)
+    (upd st 2ul v);
+
+  let v =
+    rst_frame both_st (fun _ -> both_st) (array_resource st)
+    (index ost 3ul) in
+
+  rst_frame both_st (fun _ -> both_st) (array_resource ost)
+    (upd st 3ul v);
+
+  let v =
+    rst_frame both_st (fun _ -> both_st) (array_resource st)
+    (index ost 4ul) in
+
+  rst_frame both_st (fun _ -> both_st) (array_resource ost)
+    (upd st 4ul v);
+
+  let v =
+    rst_frame both_st (fun _ -> both_st) (array_resource st)
+    (index ost 5ul) in
+
+  rst_frame both_st (fun _ -> both_st) (array_resource ost)
+    (upd st 5ul v);
+
+  let v =
+    rst_frame both_st (fun _ -> both_st) (array_resource st)
+    (index ost 6ul) in
+
+  rst_frame both_st (fun _ -> both_st) (array_resource ost)
+    (upd st 6ul v);
+
+  let v =
+    rst_frame both_st (fun _ -> both_st) (array_resource st)
+    (index ost 7ul) in
+
+  rst_frame both_st (fun _ -> both_st) (array_resource ost)
+    (upd st 7ul v);
+
+  let v =
+    rst_frame both_st (fun _ -> both_st) (array_resource st)
+    (index ost 8ul) in
+
+  rst_frame both_st (fun _ -> both_st) (array_resource ost)
+    (upd st 8ul v);
+
+  let v =
+    rst_frame both_st (fun _ -> both_st) (array_resource st)
+    (index ost 9ul) in
+
+  rst_frame both_st (fun _ -> both_st) (array_resource ost)
+    (upd st 9ul v);
+
+  let v =
+    rst_frame both_st (fun _ -> both_st) (array_resource st)
+    (index ost 10ul) in
+
+  rst_frame both_st (fun _ -> both_st) (array_resource ost)
+    (upd st 10ul v);
+
+  let v =
+    rst_frame both_st (fun _ -> both_st) (array_resource st)
+    (index ost 11ul) in
+
+  rst_frame both_st (fun _ -> both_st) (array_resource ost)
+    (upd st 11ul v);
+
+  let v =
+    rst_frame both_st (fun _ -> both_st) (array_resource st)
+    (index ost 12ul) in
+
+  rst_frame both_st (fun _ -> both_st) (array_resource ost)
+    (upd st 12ul v);
+
+  let v =
+    rst_frame both_st (fun _ -> both_st) (array_resource st)
+    (index ost 13ul) in
+
+  rst_frame both_st (fun _ -> both_st) (array_resource ost)
+    (upd st 13ul v);
+
+  let v =
+    rst_frame both_st (fun _ -> both_st) (array_resource st)
+    (index ost 14ul) in
+
+  rst_frame both_st (fun _ -> both_st) (array_resource ost)
+    (upd st 14ul v);
+
+  let v =
+    rst_frame both_st (fun _ -> both_st) (array_resource st)
+    (index ost 15ul) in
+
+  rst_frame both_st (fun _ -> both_st) (array_resource ost)
+    (upd st 15ul v);
+
+  let h1 = rst_get both_st in
+
+  //assert False;
+  Seq.lemma_eq_intro (as_rseq st h1) (as_rseq ost h0)
